validity of empty, nat and sigma

theories/Substitution/Introductions/Nat.v
@@ -1,8 +1,8 @@
 From LogRel.AutoSubst Require Import core unscoped Ast Extra.
 From LogRel Require Import Utils BasicAst Notations Context NormalForms Weakening GenericTyping LogicalRelation Validity.
-From LogRel.LogicalRelation Require Import Induction Irrelevance Escape Reflexivity Weakening Neutral Transitivity Reduction Application Universe SimpleArr.
-From LogRel.Substitution Require Import Irrelevance Properties Conversion SingleSubst Reflexivity.
-From LogRel.Substitution.Introductions Require Import Universe Pi SimpleArr Var.
+From LogRel.LogicalRelation Require Import Induction  Escape Irrelevance Reflexivity Irrelevance Weakening Neutral Transitivity Reduction Application Universe EqRedRight SimpleArr.
+From LogRel.Substitution Require Import Irrelevance Properties Conversion SingleSubst Reflexivity Reduction.
+From LogRel.Substitution.Introductions Require Import Universe Pi SimpleArr Var Application.
 
 Set Universe Polymorphism.
 
@@ -13,7 +13,7 @@ Set Printing Primitive Projection Parameters.
 
 
 Lemma natRed {Γ l} : [|- Γ] -> [Γ ||-<l> tNat].
-Proof. 
+Proof.
   intros; eapply LRNat_; constructor; eapply redtywf_refl; gen_typing.
 Defined.
 
@@ -24,7 +24,7 @@ Proof.
   + cbn; constructor; eapply redtywf_refl; gen_typing.
 Defined.
 
-Lemma natconvValid {Γ l} (VΓ : [||-v Γ]) (VNat : [Γ ||-v<l> tNat | VΓ]) : 
+Lemma natconvValid {Γ l} (VΓ : [||-v Γ]) (VNat : [Γ ||-v<l> tNat | VΓ]) :
   [Γ ||-v<l> tNat ≅ tNat | VΓ | VNat].
 Proof.
   constructor; intros.
@@ -32,197 +32,94 @@ Proof.
   constructor; cbn; eapply redtywf_refl; gen_typing.
 Qed.
 
-Lemma redUOne {Γ} : [|- Γ] -> [Γ ||-U<one> U].
+Lemma natURedTm {Δ} (wfΔ : [|-Δ]) : URedTm (LogRelRec one) Δ tNat U (redUOneCtx wfΔ).
 Proof.
-  intros ; econstructor; [easy| gen_typing|eapply redtywf_refl; gen_typing].
+  exists tNat; [| constructor].
+  eapply redtmwf_refl; gen_typing.
 Defined.
 
-Lemma natTermRed {Δ} (wfΔ : [|-Δ]) : [Δ ||-<one> tNat : U | LRU_ (redUOne wfΔ)].
+Lemma natTermRed {Δ} (wfΔ : [|-Δ]) : [Δ ||-<one> tNat : U | LRU_ (redUOneCtx wfΔ)].
 Proof.
-  econstructor.
-  + eapply redtmwf_refl; gen_typing.
-  + constructor.
-  + gen_typing.
-  + now eapply (natRed (l:= zero)).
+  unshelve eexists (natURedTm wfΔ) (natURedTm wfΔ) _; cbn.
+  1,3: now eapply (natRed (l:=zero)).
+  1: gen_typing.
+  apply reflLRTyEq.
 Defined.
 
 Lemma natTermValid {Γ} (VΓ : [||-v Γ]):  [Γ ||-v<one> tNat : U | VΓ | UValid VΓ].
 Proof.
-  constructor; intros.
-  - eapply natTermRed. 
-  - eexists (natTermRed wfΔ) (natTermRed wfΔ) (natRed wfΔ); cbn.
-    + gen_typing.
-    + now eapply (natRed (l:=zero)).
-    + constructor; eapply redtywf_refl; gen_typing.
+  constructor; intros; eapply natTermRed.
 Qed.
 
 Lemma zeroRed {Γ l} {NN : [Γ ||-Nat tNat]} (wfΓ : [|- Γ]): [Γ ||-<l> tZero : _ | LRNat_ l NN].
-Proof.
-  exists tZero.
-  1,2: gen_typing.
-  constructor.
-Defined.
-
-Lemma zeroRedEq {Γ l} {NN : [Γ ||-Nat tNat]} (wfΓ : [|- Γ]): [Γ ||-<l> tZero ≅ tZero : _ | LRNat_ l NN].
 Proof.
   exists tZero tZero.
   1-3: gen_typing.
   constructor.
 Defined.
 
-Lemma zeroValid {Γ l} (VΓ : [||-v Γ]): 
+Lemma zeroRedEq {Γ l} {NN : [Γ ||-Nat tNat]} (wfΓ : [|- Γ]): [Γ ||-<l> tZero ≅ tZero : _ | LRNat_ l NN].
+Proof. now apply zeroRed. Defined.
+
+Lemma zeroValid {Γ l} (VΓ : [||-v Γ]):
   [Γ ||-v<l> tZero : tNat | VΓ | natValid VΓ].
 Proof.
-  constructor; intros; cbn; [unshelve eapply zeroRed| unshelve eapply zeroRedEq]; tea.
+  constructor; intros; cbn; unshelve eapply zeroRed; tea.
 Qed.
+
+Lemma succRedEq {Γ l n n'} {NN : [Γ ||-Nat tNat]} :
+  [Γ ||-<l> n ≅ n' : _ | LRNat_ l NN] ->
+  [Γ ||-<l> tSucc n ≅ tSucc n' : _ | LRNat_ l NN].
+Proof.
+  intros h; pose proof (h' :=h); inversion h'; subst.
+  escape; exists (tSucc n) (tSucc n').
+  1,2: eapply redtmwf_refl; eapply ty_succ; gen_typing.
+  + eapply convtm_succ; eapply convtm_exp; gen_typing.
+  + now constructor.
+Defined.
 
 Lemma succRed {Γ l n} {NN : [Γ ||-Nat tNat]} :
   [Γ ||-<l> n : _ | LRNat_ l NN] ->
   [Γ ||-<l> tSucc n : _ | LRNat_ l NN].
-Proof.
-  intros Rn; exists (tSucc n).
-  + eapply redtmwf_refl; eapply ty_succ; now escape.
-  + eapply convtm_succ; eapply escapeEqTerm; now eapply reflLRTmEq.
-  + now constructor.
-Defined.
+Proof. eapply succRedEq. Defined.
 
-Lemma succRedEq {Γ l n n'} {NN : [Γ ||-Nat tNat]} :
-  [Γ ||-<l> n : _ | LRNat_ l NN] ->
-  [Γ ||-<l> n' : _ | LRNat_ l NN] ->
-  [Γ ||-<l> n ≅ n' : _ | LRNat_ l NN] ->
-  [Γ ||-<l> tSucc n ≅ tSucc n' : _ | LRNat_ l NN].
-Proof.
-  intros ???; escape; exists (tSucc n) (tSucc n').
-  1,2: eapply redtmwf_refl; now eapply ty_succ.
-  + now eapply convtm_succ.
-  + now constructor.
-Defined.
 
-Lemma succRedInv {Γ l n} {NN : [Γ ||-Nat tNat]} :
-  [Γ ||-<l> tSucc n : _ | LRNat_ l NN] ->
-  [Γ ||-<l> n : _ | LRNat_ l NN].
+Lemma succRedInv {Γ l n m } {NN : [Γ ||-Nat tNat]} :
+  [Γ ||-<l> tSucc n ≅ tSucc m : _ | LRNat_ l NN] ->
+  [Γ ||-<l> n ≅ m : _ | LRNat_ l NN].
 Proof.
-  intros RSn; inversion RSn; subst. 
-  unshelve epose proof (redtmwf_whnf red _). 1: constructor.
+  intros RSn; inversion RSn; subst.
+  unshelve epose proof (redtmwf_whnf redL _); try constructor.
+  unshelve epose proof (redtmwf_whnf redR _); try constructor.
   subst. inversion prop; subst; tea.
-  match goal with H : [ _ ||-NeNf _ : _] |- _ => destruct H; apply convneu_whne in refl; inv_whne end.
+  match goal with H : [ _ ||-NeNf _ ≅ _ : _] |- _ => destruct H as [?? refl] end.
+  apply convneu_whne in refl; inv_whne.
 Qed.
 
-Lemma succValid {Γ l n} (VΓ : [||-v Γ]) 
-  (Vn : [Γ ||-v<l> n : tNat | VΓ | natValid VΓ]) :
-  [Γ ||-v<l> tSucc n : tNat | VΓ | natValid VΓ].
-Proof.
-  constructor; intros; cbn.
-  - instValid Vσ ; now unshelve eapply succRed.
-  - instAllValid Vσ Vσ' Vσσ'; now unshelve eapply succRedEq.
-Qed.
 
-Lemma succcongValid {Γ l n n'} (VΓ : [||-v Γ]) 
-  (Vn : [Γ ||-v<l> n : tNat | VΓ | natValid VΓ])
-  (Vn' : [Γ ||-v<l> n' : tNat | VΓ | natValid VΓ])
+Lemma succcongValid {Γ l n n'} (VΓ : [||-v Γ])
   (Veqn : [Γ ||-v<l> n ≅ n' : tNat | VΓ | natValid VΓ]) :
   [Γ ||-v<l> tSucc n ≅ tSucc n' : tNat | VΓ | natValid VΓ].
 Proof.
-  constructor; intros; cbn; instValid Vσ; now unshelve eapply succRedEq.
+  constructor; intros; cbn; instValid Vσσ'; now unshelve eapply succRedEq.
 Qed.
 
+Lemma succValid {Γ l n} (VΓ : [||-v Γ])
+  (Vn : [Γ ||-v<l> n : tNat | VΓ | natValid VΓ]) :
+  [Γ ||-v<l> tSucc n : tNat | VΓ | natValid VΓ].
+Proof. now eapply lreflValidTm, succcongValid, reflValidTm. Qed.
 
 Lemma elimSuccHypTy_subst {P} σ :
   elimSuccHypTy P[up_term_term σ] = (elimSuccHypTy P)[σ].
 Proof.
   unfold elimSuccHypTy.
   cbn. rewrite shift_up_eq.
-  rewrite liftSubstComm. cbn. 
+  rewrite liftSubstComm. cbn.
   now rewrite up_liftSubst_eq.
 Qed.
 
 Lemma liftSubst_singleSubst_eq {t u v: term} : t[u]⇑[v..] = t[u[v..]..].
 Proof. now bsimpl. Qed.
-
-Definition natElim {Γ A} (P hz hs : term) {n} {NA : [Γ ||-Nat A]} (p : NatProp NA n) : term.
-Proof.
-  destruct p.
-  - exact hz.
-  - exact (tApp (tApp hs n) (tNatElim P hz hs n)).
-  - exact (tNatElim P hz hs ne).
-Defined.
-
-Section NatElimRed.
-  Context {Γ l P hs hz}
-    (wfΓ : [|- Γ])
-    (NN : [Γ ||-Nat tNat])
-    (RN := LRNat_ _ NN)
-    (RP : [Γ,, tNat ||-<l> P])
-    (RPpt : forall n, [Γ ||-<l> n : _ | RN] -> [Γ ||-<l> P[n..]])
-    (RPext : forall n n' (Rn : [Γ ||-<l> n : _ | RN]),
-      [Γ ||-<l> n' : _ | RN] ->
-      [Γ ||-<l> n ≅ n' : _ | RN] ->
-      [Γ ||-<l> P[n..] ≅ P[n'..] | RPpt _ Rn])
-    (RPz := RPpt _ (zeroRed wfΓ))
-    (Rhz : [Γ ||-<l> hz : P[tZero..] | RPz]) 
-    (RPs : [Γ ||-<l> elimSuccHypTy P])
-    (Rhs : [Γ ||-<l> hs : _ | RPs]).
-
-  Definition natRedElimStmt :=
-    (forall n (Rn : [Γ ||-<l> n : _ | RN]), 
-      [Γ ||-<l> tNatElim P hz hs n : _ | RPpt _ Rn ] ×
-      [Γ ||-<l> tNatElim P hz hs n ≅ tNatElim P hz hs (NatRedTm.nf Rn) : _ | RPpt _ Rn]) ×
-    (forall n (Nn : NatProp NN n) (Rn : [Γ ||-<l> n : _ | RN]), 
-      [Γ ||-<l> tNatElim P hz hs n : _ | RPpt _ Rn ] ×
-      [Γ ||-<l> tNatElim P hz hs n ≅ natElim P hz hs Nn : _ | RPpt _ Rn]).
-
-  Lemma natElimRedAux : natRedElimStmt.
-  Proof.
-    escape.
-    apply NatRedInduction.
-    - intros ? nf red ? nfprop ih.
-      assert [Γ ||-<l> nf : _ | RN]. 1:{
-        econstructor; tea.
-        eapply redtmwf_refl; gen_typing.
-      }
-      eapply redSubstTerm.
-      + eapply LRTmRedConv. 
-        2: unshelve eapply ih; tea.
-        eapply RPext. 
-        2: eapply LRTmEqSym.
-        1,2: eapply redwfSubstTerm; tea.
-      + eapply redtm_natelim; tea.
-        cbn; gen_typing.
-    - intros. 
-      eapply redSubstTerm.
-      2: eapply redtm_natElimZero; tea.
-      irrelevance.
-    - intros n Rn ih RSucc; change [Γ ||-<l> n : tNat | RN] in Rn.
-      eapply redSubstTerm.
-      2: eapply redtm_natElimSucc; tea.
-      2: now escape.
-      eapply simple_appTerm.
-      2: eapply ih.
-      irrelevance0.
-      2: unshelve eapply (appTerm RPs Rhs Rn).
-      now bsimpl.
-    - intros ? [] ?.
-      apply reflect.
-      + apply completeness.
-      + now eapply ty_natElim.
-      + now eapply ty_natElim.
-      + eapply convneu_natElim; tea.
-        { eapply escapeEq, reflLRTyEq. }
-        { eapply escapeEqTerm; now eapply reflLRTmEq. }
-        { eapply escapeEqTerm; now eapply reflLRTmEq. }
-    Unshelve.
-    * eapply ArrRedTy; now eapply RPpt.
-    * rewrite subst_arr. eapply ArrRedTy.
-      2: rewrite liftSubst_singleSubst_eq; cbn.
-      all: now eapply RPpt.
-    * exact l.
-    * assumption.
-  Qed.
-
-  Lemma natElimRed : forall n (Rn : [Γ ||-<l> n : _ | RN]), [Γ ||-<l> tNatElim P hz hs n : _ | RPpt _ Rn ].
-  Proof. intros. apply (fst natElimRedAux). Qed.
-End NatElimRed.
-
 
 Section NatElimRedEq.
   Context {Γ l P Q hs hs' hz hz'}
@@ -232,128 +129,94 @@ Section NatElimRedEq.
     (RP : [Γ,, tNat ||-<l> P])
     (RQ : [Γ,, tNat ||-<l> Q])
     (eqPQ : [Γ,, tNat |- P ≅ Q])
-    (RPpt : forall n, [Γ ||-<l> n : _ | RN] -> [Γ ||-<l> P[n..]])
-    (RQpt : forall n, [Γ ||-<l> n : _ | RN] -> [Γ ||-<l> Q[n..]])
-    (RPQext : forall n n' (Rn : [Γ ||-<l> n : _ | RN]),
-      [Γ ||-<l> n' : _ | RN] ->
-      [Γ ||-<l> n ≅ n' : _ | RN] ->
-      [Γ ||-<l> P[n..] ≅ Q[n'..] | RPpt _ Rn])
-    (RPz := RPpt _ (zeroRed wfΓ))
-    (RQz := RQpt _ (zeroRed wfΓ))
-    (Rhz : [Γ ||-<l> hz : P[tZero..] | RPz]) 
-    (RQhz : [Γ ||-<l> hz' : Q[tZero..] | RQz]) 
-    (RPQhz : [Γ ||-<l> hz ≅ hz' : _ | RPz])
+    (RPpt : forall n n', [Γ ||-<l> n ≅ n' : _ | RN] -> [Γ ||-<l> P[n..]])
+    (* (RQpt : forall n n', [Γ ||-<l> n ≅ n': _ | RN] -> [Γ ||-<l> Q[n..]]) *)
+    (RPQext : forall n n' (Rn : [Γ ||-<l> n ≅ n' : _ | RN]),
+      [Γ ||-<l> P[n..] ≅ Q[n'..] | RPpt _ _ Rn])
+    (RPz := RPpt _ _ (zeroRed wfΓ))
+    (RPQz := RPQext _ _ (zeroRedEq wfΓ))
+    (Rhz : [Γ ||-<l> hz ≅ hz' : _ | RPz])
     (RPs : [Γ ||-<l> elimSuccHypTy P])
     (RQs : [Γ ||-<l> elimSuccHypTy Q])
-    (Rhs : [Γ ||-<l> hs : _ | RPs])
-    (RQhs : [Γ ||-<l> hs' : _ | RQs])
-    (RPQhs : [Γ ||-<l> hs ≅ hs' : _ | RPs ])
+    (RPQs : [Γ ||-<l> elimSuccHypTy P ≅ elimSuccHypTy Q | RPs])
+    (Rhs : [Γ ||-<l> hs ≅ hs' : _ | RPs ])
     .
 
-  Lemma RPext : forall n n' (Rn : [Γ ||-<l> n : _ | RN]),
-      [Γ ||-<l> n' : _ | RN] ->
-      [Γ ||-<l> n ≅ n' : _ | RN] ->
-      [Γ ||-<l> P[n..] ≅ P[n'..] | RPpt _ Rn].
-  Proof.
-    intros. eapply transEq; [| eapply LRTyEqSym ]; eapply RPQext; cycle 1; tea.
-    now eapply reflLRTmEq.
-    Unshelve. 2,3: eauto.
-  Qed.
+  #[local]
+  Lemma RQpt : forall n n', [Γ ||-<l> n ≅ n': _ | RN] -> [Γ ||-<l> Q[n..]].
+  Proof. intros; now unshelve eapply LRTyEqRedRight, RPQext. Qed.
 
-  Lemma natElimRedAuxLeft : @natRedElimStmt _ _ P hs hz NN RPpt.
-  Proof.
-    eapply natElimRedAux; tea.
-    + eapply RPext.
-  Qed.
+  Let RQz := RQpt _ _ (zeroRed wfΓ).
 
-  Lemma natElimRedAuxRight : @natRedElimStmt _ _ Q hs' hz' NN RQpt.
+  #[local]
+  Lemma RPext : forall n n' (Rn : [Γ ||-<l> n ≅ n' : _ | RN]),
+      [Γ ||-<l> P[n..] ≅ P[n'..] | RPpt _ _ Rn].
   Proof.
-    eapply natElimRedAux; tea.
-    + intros. eapply transEq; [eapply LRTyEqSym |]; eapply RPQext; cycle 1; tea.
-      now eapply reflLRTmEq.
-    Unshelve. all:tea.
+    intros; eapply transEq; [| eapply LRTyEqSym ].
+    all: unshelve (eapply RPQext; cycle 1; tea); now eapply urefl.
+    Unshelve. 2: eapply RQpt; now symmetry.
   Qed.
 
   Lemma natElimRedEqAux :
-    (forall n n' (Rnn' : [Γ ||-<l> n ≅ n' : _ | RN]) (Rn : [Γ ||-<l> n : _ | RN]) (Rn' : [Γ ||-<l> n' : _ | RN]), 
-      [Γ ||-<l> tNatElim P hz hs n ≅ tNatElim Q hz' hs' n' : _ | RPpt _ Rn ]) ×
-    (forall n n' (Rnn' : NatPropEq NN n n') (Rn : [Γ ||-<l> n : _ | RN]) (Rn' : [Γ ||-<l> n' : _ | RN]), 
-      [Γ ||-<l> tNatElim P hz hs n ≅ tNatElim Q hz' hs' n' : _ | RPpt _ Rn ]).
+    (forall n n' (Rnn' : [Γ ||-<l> n ≅ n' : _ | RN]), [Γ ||-<l> n ≅ n' : _ | RN] ->
+      [Γ ||-<l> tNatElim P hz hs n ≅ tNatElim Q hz' hs' n' : _ | RPpt _ _ Rnn' ]) ×
+    (forall n n' (Rnn' : NatPropEq NN n n') (RP : [Γ ||-<l> P[n..]]),
+    (* (Rn : [Γ ||-<l> n ≅ n' : _ | RN]), *)
+      [Γ ||-<l> tNatElim P hz hs n ≅ tNatElim Q hz' hs' n' : _ | RP (*RPpt _ _ Rn*) ]).
   Proof.
     apply NatRedEqInduction.
-    - intros ?? nfL nfR redL redR ? prop ih RL RR; destruct (NatPropEq_whnf prop).
-      assert [Γ ||-<l> nfL : _ | RN] by (eapply redTmFwd; cycle 1; tea).
-      assert [Γ ||-<l> nfR : _ | RN] by (eapply redTmFwd; cycle 1; tea).
-      eapply LREqTermHelper.
-      * eapply (fst natElimRedAuxLeft).
-      * eapply (fst natElimRedAuxRight).
-      * eapply RPQext. 1: tea.
-        now econstructor.
-      * eapply LRTmEqRedConv.
-        + eapply RPext; tea. 
-          eapply LRTmEqSym; eapply redwfSubstTerm; cycle 1; tea.
-        + unshelve erewrite (redtmwf_det _ _ (NatRedTm.red RL) redL); tea.
-          1: dependent inversion RL; subst; cbn; now eapply NatProp_whnf.
-          unshelve erewrite (redtmwf_det _ _ (NatRedTm.red RR) redR); tea.
-          1: dependent inversion RR; subst; cbn; now eapply NatProp_whnf.
-          now eapply ih.
-        Unshelve. tea.
-    - intros. eapply LREqTermHelper.
-      * unshelve eapply (snd natElimRedAuxLeft); constructor.
-      * unshelve eapply (snd natElimRedAuxRight); tea; constructor.
-      * eapply RPQext; [unshelve eapply zeroRed| unshelve eapply zeroRedEq]; tea.
-      * cbn; irrelevance.
-    - intros ??? ih Rn Rn'. pose proof (succRedInv Rn); pose proof (succRedInv Rn').
-      eapply LREqTermHelper.
-      * unshelve eapply (snd natElimRedAuxLeft); now constructor.
-      * unshelve eapply (snd natElimRedAuxRight); tea; now constructor.
-      * eapply RPQext; [unshelve eapply succRed| unshelve eapply succRedEq]; tea.
-      * cbn.
-        eapply simple_appcongTerm.
-        4: now eapply ih.
-        + irrelevance0. 2: eapply appcongTerm; tea.
-          now bsimpl.
-        + eapply (fst natElimRedAuxLeft).
-        + eapply LRTmRedConv. 2: eapply (fst natElimRedAuxRight).
-          eapply LRTyEqSym; now eapply RPQext.
-        Unshelve. 2,4,5: tea.
-        1: eapply ArrRedTy; now eapply RPpt.
-        rewrite subst_arr. eapply ArrRedTy.
-        2: rewrite liftSubst_singleSubst_eq; cbn.
-        all: now eapply RPpt.
-    - intros ?? neueq ??. escape. inversion neueq.
-      assert [Γ |- P[ne..] ≅ Q[ne'..]]. 1:{
-        eapply escapeEq. eapply RPQext; tea.
-        econstructor.
-        1,2: now eapply redtmwf_refl.
-        2: now constructor.
-        gen_typing.
-      }
-      eapply neuTermEq.
-      + eapply ty_natElim; tea.
-      + eapply ty_conv. 
-        1: eapply ty_natElim; tea.
-        now symmetry.
-      + eapply convneu_natElim ; tea.
-      Unshelve. tea.
+    - intros ?? nfL nfR redL redR ? prop ih Rtu ; destruct (NatPropEq_whnf prop).
+      eapply redSubstTmEq.
+      + eapply LRTmEqConv, ih; unshelve eapply RPext.
+        eapply redTmEqFwd; tea; now eapply lrefl.
+      + escape; eapply redtm_natelim; tea; gen_typing.
+      + escape; eapply redtm_natelim; tea; [..| gen_typing].
+        1,2: now eapply ty_conv.
+      + now unshelve eapply escapeEq, RPQext.
+    - intros. eapply redSubstTmEq.
+      + irrelevanceRefl; eapply Rhz.
+      + escape; eapply redtm_natElimZero; tea.
+      + escape; eapply redtm_natElimZero; tea.
+        1,2: now eapply ty_conv.
+      + now escape.
+    - intros n n' Rn ih ?; change [Γ ||-<l> n ≅ n' : _ | RN] in Rn.
+      eapply redSubstTmEq; cycle 1.
+      + escape; eapply redtm_natElimSucc; tea.
+      + escape; eapply redtm_natElimSucc; tea.
+        1,2: now eapply ty_conv.
+      + unshelve eapply escapeEq, RPQext.
+        now eapply succRedEq.
+      + assert [Γ ||-<l> arr P[n..] P[(tSucc n)..]].
+        1: now (eapply ArrRedTy; eapply RPpt; [| eapply succRedEq]).
+        unshelve eapply simple_appcongTerm; [..| eauto]; tea.
+        unshelve (irrelevance0; [| eapply appcongTerm; tea]).
+        all: now rewrite subst_arr, liftSubst_singleSubst_eq.
+    - intros n n' Rn RP0.
+      pose proof (neNfTermEq RN Rn).
+      eapply neuTermEq. 2: eapply ty_conv ; [| eapply escapeEq; eapply LRTyEqSym].
+      + escape; now eapply ty_natElim.
+      + escape; eapply ty_natElim; tea.
+        all: now eapply ty_conv.
+      + now unshelve eapply RPQext.
+      + escape ; destruct Rn; now eapply convneu_natElim.
+      Unshelve. 2: eapply RQpt; now eapply urefl.
   Qed.
 
   Lemma natElimRedEq :
-    (forall n n' (Rnn' : [Γ ||-<l> n ≅ n' : _ | RN]) (Rn : [Γ ||-<l> n : _ | RN]) (Rn' : [Γ ||-<l> n' : _ | RN]), 
-      [Γ ||-<l> tNatElim P hz hs n ≅ tNatElim Q hz' hs' n' : _ | RPpt _ Rn ]).
-  Proof. apply natElimRedEqAux. Qed.
+    (forall n n' (Rnn' : [Γ ||-<l> n ≅ n' : _ | RN]),
+      [Γ ||-<l> tNatElim P hz hs n ≅ tNatElim Q hz' hs' n' : _ | RPpt _ _ Rnn' ]).
+  Proof. intros; now apply (fst natElimRedEqAux). Qed.
 End NatElimRedEq.
 
 
-
 Section NatElimValid.
-  Context {Γ l P}
+  Context {Γ l}
     (VΓ : [||-v Γ])
     (VN := natValid (l:=l) VΓ)
-    (VΓN := validSnoc VΓ VN)
-    (VP : [Γ ,, tNat ||-v<l> P | VΓN]).
-  
-  Lemma elimSuccHypTyValid :
+    (VΓN := validSnoc VΓ VN).
+
+  Lemma elimSuccHypTyValid {P}
+    (VP : [Γ ,, tNat ||-v<l> P | VΓN]) :
     [Γ ||-v<l> elimSuccHypTy P | VΓ].
   Proof.
     unfold elimSuccHypTy.
@@ -367,183 +230,14 @@ Section NatElimValid.
     change tNat with tNat⟨@wk1 Γ tNat⟩ at 2.
     eapply var0Valid.
     Unshelve. all: tea.
-  Qed.
+  Defined.
 
-  Context {hz hs}
-    (VPz := substS VP (zeroValid VΓ))
-    (Vhz : [Γ ||-v<l> hz : P[tZero..] | VΓ | VPz]) 
-    (Vhs : [Γ ||-v<l> hs : _ | VΓ | elimSuccHypTyValid]).
-
-
-  Lemma natElimValid {n}
-    (Vn : [Γ ||-v<l> n : tNat | VΓ | VN])
-    (VPn := substS VP Vn)
-    : [Γ ||-v<l> tNatElim P hz hs n : _ | VΓ | VPn].
+  Lemma elimSuccHypTyCongValid {P P'}
+      (VP : [Γ ,, tNat ||-v<l> P | VΓN])
+      (VeqP : [Γ ,, tNat ||-v<l> P ≅ P' | VΓN | VP ]) :
+      [Γ ||-v<l> elimSuccHypTy P ≅ elimSuccHypTy P' | VΓ | elimSuccHypTyValid VP].
   Proof.
-    constructor; intros.
-    - instValid Vσ; cbn.
-      irrelevance0.  1: now rewrite singleSubstComm'.
-      epose proof (Vuσ := liftSubstS' VN Vσ).
-      instValid Vuσ; escape.
-      unshelve eapply natElimRed; tea.
-      + intros m Rm.
-        rewrite up_single_subst. 
-        unshelve eapply validTy; cycle 1; tea.
-        unshelve econstructor; [now bsimpl| now cbn].
-      + rewrite elimSuccHypTy_subst. eapply validTy; tea; eapply elimSuccHypTyValid.
-      + intros m m' Rm Rm' Rmm'; cbn.
-        irrelevance0. 1: now rewrite up_single_subst.
-        rewrite up_single_subst.
-        unshelve eapply validTyExt; cycle 1 ; tea.
-        1,2: unshelve econstructor; [now bsimpl| now cbn].
-        unshelve econstructor; [|now cbn].
-        bsimpl; cbn; eapply reflSubst.
-      + irrelevance.
-      + irrelevance. now rewrite elimSuccHypTy_subst. 
-    - instAllValid Vσ Vσ' Vσσ'.
-      irrelevance0.  1: now rewrite singleSubstComm'.
-      pose (Vuσ := liftSubstS' VN Vσ).
-      pose proof (Vuσ' := liftSubstS' VN Vσ').
-      pose proof (Vuσrea :=  liftSubstSrealign' VN Vσσ' Vσ').
-      pose proof (Vuσσ' := liftSubstSEq' VN Vσσ').
-      instValid Vuσ'; instAllValid Vuσ Vuσrea Vuσσ'; escape.
-      unshelve eapply natElimRedEq; tea; fold subst_term.
-      6-11: irrelevance; now rewrite elimSuccHypTy_subst.
-      3,4: rewrite elimSuccHypTy_subst; eapply validTy; tea; eapply elimSuccHypTyValid.
-      + intros m Rm.
-        rewrite up_single_subst. 
-        unshelve eapply validTy; cycle 1; tea.
-        unshelve econstructor; [now bsimpl| now cbn].
-      + intros m Rm.
-        rewrite up_single_subst. 
-        unshelve eapply validTy; cycle 1; tea.
-        unshelve econstructor; [now bsimpl| now cbn].
-      + intros m m' Rm Rm' Rmm'; cbn.
-        irrelevance0. 1: now rewrite up_single_subst.
-        rewrite up_single_subst.
-        unshelve eapply validTyExt; cycle 1 ; tea.
-        1,2: unshelve econstructor; [now bsimpl| now cbn].
-        unshelve econstructor; [|now cbn].
-        now bsimpl.
-  Qed.
-
-  Lemma natElimZeroValid  : 
-    [Γ ||-v<l> tNatElim P hz hs tZero ≅ hz : _ | VΓ | VPz].
-  Proof.
-    constructor; intros.
-    epose proof (Vuσ := liftSubstS' VN Vσ).
-    instValid Vσ; instValid Vuσ; escape.
-    irrelevance0.  1: now rewrite singleSubstComm'.
-    unshelve eapply (snd (natElimRedAux _ _ _ _ _ _ _ _) _ NatRedTm.zeroR); tea; fold subst_term.
-    7: eapply zeroValid.
-    + intros m Rm.
-      rewrite up_single_subst. 
-      unshelve eapply validTy; cycle 1; tea.
-      unshelve econstructor; [now bsimpl| now cbn].
-    + intros m m' Rm Rm' Rmm'; cbn.
-      irrelevance0. 1: now rewrite up_single_subst.
-      rewrite up_single_subst.
-      unshelve eapply validTyExt; cycle 1 ; tea.
-      1,2: unshelve econstructor; [now bsimpl| now cbn].
-      unshelve econstructor; [|now cbn].
-      bsimpl; cbn; eapply reflSubst.
-    + irrelevance.
-    + rewrite elimSuccHypTy_subst. eapply validTy; tea; eapply elimSuccHypTyValid.
-    + irrelevance. now rewrite elimSuccHypTy_subst. 
-    Unshelve. 4: tea.
-  Qed.
-
-  Lemma natElimSuccValid {n}
-    (Vn : [Γ ||-v<l> n : tNat | VΓ | VN]) 
-    (VPSn := substS VP (succValid _ Vn)) : 
-    [Γ ||-v<l> tNatElim P hz hs (tSucc n) ≅ tApp (tApp hs n) (tNatElim P hz hs n) : _ | VΓ | VPSn].
-  Proof.
-    constructor; intros.
-    epose proof (Vuσ := liftSubstS' VN Vσ).
-    instValid Vσ; instValid Vuσ; escape.
-    irrelevance0.  1: now rewrite singleSubstComm'.
-    pose (NSn := NatRedTm.succR RVn).
-    unshelve eapply (snd (natElimRedAux _ _ _ _ _ _ _ _) _ NSn); tea; fold subst_term.
-    + intros m Rm.
-      rewrite up_single_subst. 
-      unshelve eapply validTy; cycle 1; tea.
-      unshelve econstructor; [now bsimpl| now cbn].
-    + intros m m' Rm Rm' Rmm'; cbn.
-      irrelevance0. 1: now rewrite up_single_subst.
-      rewrite up_single_subst.
-      unshelve eapply validTyExt; cycle 1 ; tea.
-      1,2: unshelve econstructor; [now bsimpl| now cbn].
-      unshelve econstructor; [|now cbn].
-      bsimpl; cbn; eapply reflSubst.
-    + irrelevance.
-    + rewrite elimSuccHypTy_subst. eapply validTy; tea; eapply elimSuccHypTyValid.
-    + irrelevance. now rewrite elimSuccHypTy_subst. 
-    + now eapply succRed.
-  Qed.
-
-End NatElimValid.
-
-Lemma natElimCongValid {Γ l P Q hz hz' hs hs' n n'}
-    (VΓ : [||-v Γ])
-    (VN := natValid (l:=l) VΓ)
-    (VΓN := validSnoc VΓ VN)
-    (VP : [Γ ,, tNat ||-v<l> P | VΓN])
-    (VQ : [Γ ,, tNat ||-v<l> Q | VΓN])
-    (VPQ : [Γ ,, tNat ||-v<l> P ≅ Q | VΓN | VP])
-    (VPz := substS VP (zeroValid VΓ))
-    (VQz := substS VQ (zeroValid VΓ))
-    (Vhz : [Γ ||-v<l> hz : P[tZero..] | VΓ | VPz]) 
-    (Vhz' : [Γ ||-v<l> hz' : Q[tZero..] | VΓ | VQz])
-    (Vheqz : [Γ ||-v<l> hz ≅ hz' : P[tZero..] | VΓ | VPz])
-    (VPs := elimSuccHypTyValid VΓ VP)
-    (VQs := elimSuccHypTyValid VΓ VQ)
-    (Vhs : [Γ ||-v<l> hs : _ | VΓ | VPs]) 
-    (Vhs' : [Γ ||-v<l> hs' : _ | VΓ | VQs])
-    (Vheqs : [Γ ||-v<l> hs ≅ hs' : _ | VΓ | VPs]) 
-    (Vn : [Γ ||-v<l> n : _ | VΓ | VN])
-    (Vn' : [Γ ||-v<l> n' : _ | VΓ | VN])
-    (Veqn : [Γ ||-v<l> n ≅ n' : _ | VΓ | VN])
-    (VPn := substS VP Vn) :
-    [Γ ||-v<l> tNatElim P hz hs n ≅ tNatElim Q hz' hs' n' : _ | VΓ | VPn].
-Proof.
-  constructor; intros.
-  pose (Vuσ := liftSubstS' VN Vσ).
-  instValid Vσ; instValid Vuσ; escape.
-  irrelevance0.  1: now rewrite singleSubstComm'.
-  unshelve eapply natElimRedEq; tea; fold subst_term.
-  6-11: irrelevance; now rewrite elimSuccHypTy_subst.
-  3,4: rewrite elimSuccHypTy_subst; eapply validTy; tea; eapply elimSuccHypTyValid.
-  + intros m Rm.
-    rewrite up_single_subst. 
-    unshelve eapply validTy; cycle 1; tea.
-    unshelve econstructor; [now bsimpl| now cbn].
-  + intros m Rm.
-    rewrite up_single_subst. 
-    unshelve eapply validTy; cycle 1; tea.
-    unshelve econstructor; [now bsimpl| now cbn].
-  + intros m m' Rm Rm' Rmm'; cbn.
-    irrelevance0. 1: now rewrite up_single_subst.
-    rewrite up_single_subst.
-    eapply transEq; cycle 1.
-    - unshelve eapply validTyEq. 
-      7: tea. 1: tea.
-      unshelve econstructor; [now bsimpl| now cbn].
-    - unshelve eapply validTyExt; cycle 1 ; tea.
-    1,2: unshelve econstructor; [now bsimpl| now cbn].
-    unshelve econstructor; [|now cbn].
-    bsimpl. eapply reflSubst.
-Qed.
-
-Lemma elimSuccHypTyCongValid {Γ l P P'}
-    (VΓ : [||-v Γ])
-    (VN := natValid (l:=l) VΓ)
-    (VΓN := validSnoc VΓ VN)
-    (VP : [Γ ,, tNat ||-v<l> P | VΓN])
-    (VP' : [Γ ,, tNat ||-v<l> P' | VΓN])
-    (VeqP : [Γ ,, tNat ||-v<l> P ≅ P' | VΓN | VP]) :
-    [Γ ||-v<l> elimSuccHypTy P ≅ elimSuccHypTy P' | VΓ | elimSuccHypTyValid VΓ VP].
-  Proof.
-    unfold elimSuccHypTy.
+    unfold elimSuccHypTy.  pose proof (ureflValidTy VeqP).
     eapply irrelevanceTyEq.
     assert [Γ,, tNat ||-v< l > P'[tSucc (tRel 0)]⇑ | validSnoc VΓ VN]. 1:{
       eapply substLiftS; tea.
@@ -566,5 +260,107 @@ Lemma elimSuccHypTyCongValid {Γ l P P'}
     1,2 : tea.
     now bsimpl.
   Qed.
+
+
+
+  Context { P P' hz hz' hs hs'}
+    (VP : [Γ ,, tNat ||-v<l> P | VΓN])
+    (VPP' : [Γ ,, tNat ||-v<l> P ≅ P' | VΓN | VP ])
+    (VP' := ureflValidTy VPP')
+    (VPz := substS VP (zeroValid VΓ))
+    (Vhz : [Γ ||-v<l> hz ≅ hz' : P[tZero..] | VΓ | VPz])
+    (Vhs : [Γ ||-v<l> hs ≅ hs' : _ | VΓ | elimSuccHypTyValid VP]).
+
+  (* Lemma elimSuccHypTyCongValid ? *)
+
+  Lemma natElimCongValid {n n'}
+    (Vn : [Γ ||-v<l> n ≅ n' : tNat | VΓ | VN])
+    (VPn := substS VP Vn)
+    : [Γ ||-v<l> tNatElim P hz hs n ≅ tNatElim P' hz' hs' n' : _ | VΓ | VPn].
+  Proof.
+    pose proof (elimSuccHypTyValid VP).
+    pose proof (elimSuccHypTyValid VP').
+    pose proof (elimSuccHypTyCongValid VP VPP').
+    constructor; intros; instValid Vσσ'; epose proof (Vuσ := liftSubstEq' VN Vσσ').
+    instValid Vuσ; cbn -[elimSuccHypTy elimSuccHypTyValid] in *; escape.
+    irrelevance0. 1: now rewrite singleSubstComm'.
+    eapply natElimRedEq; rewrite ?elimSuccHypTy_subst; tea.
+    + intros; irrelevance0; rewrite up_single_subst; [reflexivity|].
+      unshelve eapply validTyEq; cycle 1 ; tea.
+      now unshelve eapply consSubstEq.
+    + irrelevance0; [exact (singleSubstComm' _ tZero σ)|]; tea.
+    + irrelevance0; [now rewrite elimSuccHypTy_subst|]; tea.
+    + irrelevance0; [now rewrite elimSuccHypTy_subst|]; tea.
+    Unshelve.
+      2,3: tea.
+      2: now rewrite elimSuccHypTy_subst.
+      intros ?? Rn; rewrite up_single_subst.
+      unshelve eapply validTy.
+      5: tea.
+      3: unshelve eapply consSubstEq; tea.
+  Qed.
+End NatElimValid.
+
+Lemma natElimValid {Γ l P hz hz' hs hs' n n'}
+    (VΓ : [||-v Γ])
+    (VN := natValid (l:=l) VΓ)
+    (VΓN := validSnoc VΓ VN)
+    (VP : [Γ ,, tNat ||-v<l> P | VΓN])
+    (VPz := substS VP (zeroValid VΓ))
+    (Vhz : [Γ ||-v<l> hz ≅ hz' : P[tZero..] | VΓ | VPz])
+    (Vhs : [Γ ||-v<l> hs ≅ hs' : _ | VΓ | elimSuccHypTyValid VΓ VP])
+    (Vn : [Γ ||-v<l> n ≅ n' : _ | VΓ | VN])
+    (VPn := substS VP Vn):
+    [Γ ||-v<l> tNatElim P hz hs n : _ | VΓ | VPn].
+Proof.
+  eapply lreflValidTm , natElimCongValid; tea.
+  now eapply reflValidTy.
+Qed.
+
+Section NatElimRedValid.
+  Context {Γ l}
+    (VΓ : [||-v Γ])
+    (VN := natValid (l:=l) VΓ)
+    (VΓN := validSnoc VΓ VN)
+    { P P' hz hz' hs hs'}
+    (VP : [Γ ,, tNat ||-v<l> P | VΓN])
+    (VPP' : [Γ ,, tNat ||-v<l> P ≅ P' | VΓN | VP ])
+    (VP' := ureflValidTy VPP')
+    (VPz := substS VP (zeroValid VΓ))
+    (Vhz : [Γ ||-v<l> hz ≅ hz' : P[tZero..] | VΓ | VPz])
+    (Vhs : [Γ ||-v<l> hs ≅ hs' : _ | VΓ | elimSuccHypTyValid VΓ VP]).
+
+  Lemma natElimZeroValid  :
+    [Γ ||-v<l> tNatElim P hz hs tZero ≅ hz : _ | VΓ | VPz].
+  Proof.
+    eapply redSubstValid. 2: now eapply lreflValidTm.
+    constructor; intros; cbn; rewrite singleSubstComm'.
+    instValid Vσσ'; instValid (liftSubstEq' VN Vσσ'); escape.
+    eapply redtm_natElimZero; tea.
+    + now rewrite <- (singleSubstComm' _ tZero σ).
+    + now rewrite elimSuccHypTy_subst.
+  Qed.
+
+  Lemma natElimSuccValid {n}
+    (Vn : [Γ ||-v<l> n : tNat | VΓ | VN])
+    (VPSn := substS VP (succValid _ Vn)) :
+    [Γ ||-v<l> tNatElim P hz hs (tSucc n) ≅ tApp (tApp hs n) (tNatElim P hz hs n) : _ | VΓ | VPSn].
+  Proof.
+    eapply redSubstValid.
+    * constructor; intros; rewrite singleSubstComm'.
+      instValid Vσσ'; instValid (liftSubstEq' VN Vσσ'); escape.
+      eapply redtm_natElimSucc; tea; refold.
+      + now rewrite <- (singleSubstComm' _ tZero σ).
+      + now rewrite elimSuccHypTy_subst.
+    * eapply simple_appValid.
+      2: now unshelve (eapply natElimValid; tea).
+      eapply irrelevanceTm'; [| exact (appValid (lreflValidTm _ Vhs) Vn)].
+      clear; now bsimpl.
+      Unshelve.
+        eapply simpleArrValid; eapply substS; tea.
+        now eapply succValid.
+  Qed.
+
+End NatElimRedValid.
 
 End Nat.
