theories/Substitution/Conversion.v
@@ -2,7 +2,7 @@ From Coq Require Import CRelationClasses.
 From LogRel.AutoSubst Require Import core unscoped Ast Extra.
 From LogRel Require Import Utils BasicAst Notations Context NormalForms Weakening GenericTyping LogicalRelation Validity.
 From LogRel.LogicalRelation Require Import Irrelevance Escape Reflexivity Weakening Neutral.
-From LogRel.Substitution Require Import  Irrelevance Properties.
+From LogRel.Substitution Require Import  Irrelevance Properties Reflexivity.
 
 Set Universe Polymorphism.
 
@@ -12,29 +12,7 @@ Context `{GenericTypingProperties}.
 Set Printing Primitive Projection Parameters.
 
 
-Lemma conv {Γ t A B l} (VΓ : [||-v Γ])
-  (VA : [Γ ||-v<l> A | VΓ])
-  (VB : [Γ ||-v<l> B | VΓ])
-  (VeqAB : [Γ ||-v<l> A ≅ B | VΓ | VA])
-  (Vt : [Γ ||-v<l> t : A | VΓ | VA]) :
-  [Γ ||-v<l> t : B | VΓ | VB].
-Proof.
-  constructor; intros; eapply LRTmEqConv.
-  2: now unshelve now eapply validTmExt.
-  now eapply validTyEqLeft.
-Qed.
-
-Lemma convsym {Γ t A B l} (VΓ : [||-v Γ])
-  (VA : [Γ ||-v<l> A | VΓ])
-  (VB : [Γ ||-v<l> B | VΓ])
-  (VeqAB : [Γ ||-v<l> A ≅ B | VΓ | VA])
-  (Vt : [Γ ||-v<l> t : B | VΓ | VB]) :
-  [Γ ||-v<l> t : A | VΓ | VA].
-Proof.
-  eapply conv; tea; now eapply symValidTyEq.
-Qed.
-
-Lemma convEq {Γ t u A B l} (VΓ : [||-v Γ])
+Lemma conv {Γ t u A B l} (VΓ : [||-v Γ])
   (VA : [Γ ||-v<l> A | VΓ])
   (VB : [Γ ||-v<l> B | VΓ])
   (VeqAB : [Γ ||-v<l> A ≅ B | VΓ | VA])
@@ -42,9 +20,28 @@ Lemma convEq {Γ t u A B l} (VΓ : [||-v Γ])
   [Γ ||-v<l> t ≅ u : B | VΓ | VB].
 Proof.
   constructor; intros; eapply LRTmEqConv.
-  1: (unshelve now eapply validTyEqLeft); cycle 2; tea.
-  now eapply validTmEq.
+  2: now unshelve now eapply validTmEq.
+  now eapply validTyEqLeft.
 Qed.
+
+Lemma convsym {Γ t u A B l} (VΓ : [||-v Γ])
+  (VA : [Γ ||-v<l> A | VΓ])
+  (VB : [Γ ||-v<l> B | VΓ])
+  (VeqAB : [Γ ||-v<l> A ≅ B | VΓ | VA])
+  (Vt : [Γ ||-v<l> t ≅ u : B | VΓ | VB]) :
+  [Γ ||-v<l> t ≅ u : A | VΓ | VA].
+Proof.
+  eapply conv; tea; now eapply symValidTyEq.
+Qed.
+
+#[deprecated(note="Use conv")]
+Lemma convEq {Γ t u A B l} (VΓ : [||-v Γ])
+  (VA : [Γ ||-v<l> A | VΓ])
+  (VB : [Γ ||-v<l> B | VΓ])
+  (VeqAB : [Γ ||-v<l> A ≅ B | VΓ | VA])
+  (Vt : [Γ ||-v<l> t ≅ u : A | VΓ | VA]) :
+  [Γ ||-v<l> t ≅ u : B | VΓ | VB].
+Proof. now eapply conv. Qed.
 
 
 Lemma convSubstEqCtx1 {Γ Δ A B l σ σ'}
@@ -53,7 +50,6 @@ Lemma convSubstEqCtx1 {Γ Δ A B l σ σ'}
   (VΓA : [||-v Γ ,, A])
   (VΓB : [||-v Γ ,, B])
   (VA : [_ ||-v<l> A | VΓ])
-  (VB : [_ ||-v<l> B | VΓ])
   (VAB : [_ ||-v<l> A ≅ B | VΓ | VA])
   (Vσσ': [_ ||-v σ ≅ σ' : _ | VΓA | wfΔ]) :
   [_ ||-v σ ≅ σ' : _ | VΓB | wfΔ].
@@ -67,7 +63,7 @@ Proof.
   1: epose (eqTail Vσσ'); irrValid.
   eapply LRTmEqConv.
   2: irrelevanceRefl; eapply eqHead.
-  eapply validTyEqLeft; [exact VB| exact VAB].
+  eapply validTyEqLeft; [eapply ureflValidTy |]; exact VAB.
   Unshelve. 6: tea.
     3: eapply irrelevanceSubstEq; now eapply eqTail.
     tea.
@@ -78,7 +74,6 @@ Lemma convCtx1 {Γ A B P l}
   (VΓA : [||-v Γ ,, A])
   (VΓB : [||-v Γ ,, B])
   (VA : [_ ||-v<l> A | VΓ])
-  (VB : [_ ||-v<l> B | VΓ])
   (VAB : [_ ||-v<l> A ≅ B | VΓ | VA])
   (VP : [_ ||-v<l> P | VΓA]) :
   [_ ||-v<l> P | VΓB].
@@ -88,7 +83,7 @@ Proof.
   - irrelevanceRefl; unshelve eapply validTyExt.
     3,4: tea.
     eapply convSubstEqCtx1; tea; now eapply symValidTyEq.
-    Unshelve. all: tea.
+    Unshelve. all: tea; now eapply ureflValidTy.
 Qed.
 
 Lemma convEqCtx1 {Γ A B P Q l}
@@ -96,7 +91,6 @@ Lemma convEqCtx1 {Γ A B P Q l}
   (VΓA : [||-v Γ ,, A])
   (VΓB : [||-v Γ ,, B])
   (VA : [_ ||-v<l> A | VΓ])
-  (VB : [_ ||-v<l> B | VΓ])
   (VAB : [_ ||-v<l> A ≅ B | VΓ | VA])
   (VP : [_ ||-v<l> P | VΓA])
   (VPB : [_ ||-v<l> P | VΓB])
@@ -106,7 +100,9 @@ Proof.
   constructor; intros; irrelevanceRefl.
   eapply validTyEq; tea.
   Unshelve. 1: tea.
-  unshelve eapply convSubstEqCtx1; cycle 5; tea; now eapply symValidTyEq.
+  unshelve eapply convSubstEqCtx1; cycle 5; tea.
+  1: now eapply symValidTyEq.
+  now eapply ureflValidTy.
 Qed.
 
 Lemma convTmEqCtx1 {Γ A B C t u l}
@@ -114,7 +110,6 @@ Lemma convTmEqCtx1 {Γ A B C t u l}
   (VΓA : [||-v Γ ,, A])
   (VΓB : [||-v Γ ,, B])
   (VA : [_ ||-v<l> A | VΓ])
-  (VB : [_ ||-v<l> B | VΓ])
   (VC : [_ ||-v<l> C | VΓA])
   (VC' : [_ ||-v<l> C | VΓB])
   (VAB : [_ ||-v<l> A ≅ B | VΓ | VA])
@@ -123,7 +118,8 @@ Lemma convTmEqCtx1 {Γ A B C t u l}
 Proof.
   constructor; intros; irrelevanceRefl.
   (unshelve now eapply validTmEq); tea.
-  now unshelve (eapply convSubstEqCtx1; tea; now eapply symValidTyEq).
+  unshelve (eapply convSubstEqCtx1; tea; now eapply symValidTyEq).
+  now eapply ureflValidTy.
 Qed.
 
 
@@ -138,7 +134,7 @@ Lemma convSubstEqCtx2 {Γ Δ A1 B1 A2 B2 l σ σ'}
   (VA2 : [_ ||-v<l> A2 | VΓA1])
   (VB2 : [_ ||-v<l> B2 | VΓA1])
   (VAB : [_ ||-v<l> A2 ≅ B2 | VΓA1 | VA2])
-  (VB2' := convCtx1 VΓ VΓA1 VΓB1 VA1 VB1 VAB1 VB2)
+  (VB2' := convCtx1 VΓ VΓA1 VΓB1 VA1 VAB1 VB2)
   (VΓA12 := validSnoc VΓA1 VA2)
   (VΓB12 := validSnoc VΓB1 VB2')
   (Vσσ' : [_ ||-v σ ≅ σ' : _ | VΓA12 | wfΔ]) :
@@ -162,14 +158,14 @@ Lemma convSubstEqCtx2' {Γ Δ A1 B1 A2 B2 l σ σ'}
   (VΓA12 : [||-v Γ ,, A1 ,, A2])
   (VΓB12 : [||-v Γ ,, B1 ,, B2])
   (VA1 : [_ ||-v<l> A1 | VΓ])
-  (VB1 : [_ ||-v<l> B1 | VΓ])
   (VAB1 : [_ ||-v<l> A1 ≅ B1 | VΓ | VA1])
   (VA2 : [_ ||-v<l> A2 | VΓA1])
-  (VB2 : [_ ||-v<l> B2 | VΓA1])
   (VAB : [_ ||-v<l> A2 ≅ B2 | VΓA1 | VA2])
   (Vσσ' : [_ ||-v σ ≅ σ' : _ | VΓA12 | wfΔ]) :
   [_ ||-v σ ≅ σ' : _ | VΓB12 | wfΔ].
 Proof.
+  pose proof (ureflValidTy VAB1).
+  pose proof (ureflValidTy VAB).
   eapply irrelevanceSubstEq.
   eapply convSubstEqCtx2; irrValid.
   Unshelve. all: tea; irrValid.
@@ -185,7 +181,7 @@ Lemma convCtx2 {Γ A1 B1 A2 B2 P l}
   (VA2 : [_ ||-v<l> A2 | VΓA1])
   (VB2 : [_ ||-v<l> B2 | VΓA1])
   (VAB : [_ ||-v<l> A2 ≅ B2 | VΓA1 | VA2])
-  (VB2' := convCtx1 VΓ VΓA1 VΓB1 VA1 VB1 VAB1 VB2)
+  (VB2' := convCtx1 VΓ VΓA1 VΓB1 VA1 VAB1 VB2)
   (VΓA12 := validSnoc VΓA1 VA2)
   (VΓB12 := validSnoc VΓB1 VB2')
   (VP : [_ ||-v<l> P | VΓA12]) :
@@ -205,19 +201,17 @@ Qed.
 Lemma convCtx2' {Γ A1 A2 B1 B2 P l}
   (VΓ : [||-v Γ])
   (VA1 : [_ ||-v<l> A1 | VΓ])
-  (VB1 : [_ ||-v<l> B1 | VΓ])
   (VAB1 : [_ ||-v<l> A1 ≅ B1 | VΓ | VA1])
   (VΓA1 : [||-v Γ ,, A1])
-  (VΓB1 : [||-v Γ ,, B1])
   (VA2 : [_ ||-v<l> A2 | VΓA1])
-  (VB2 : [_ ||-v<l> B2 | VΓA1])
   (VAB : [_ ||-v<l> A2 ≅ B2 | VΓA1 | VA2])
-  (VB2' : [_ ||-v<l> B2 | VΓB1])
   (VΓA12 : [||-v Γ ,, A1 ,, A2])
   (VΓB12 : [||-v Γ ,, B1,, B2])
   (VP : [_ ||-v<l> P | VΓA12]) :
   [_ ||-v<l> P | VΓB12].
 Proof.
+  pose proof (ureflValidTy VAB1).
+  pose proof (ureflValidTy VAB).
   eapply irrelevanceTy; eapply convCtx2; irrValid.
   Unshelve. all: tea; irrValid.
 Qed.
