theories/Substitution/Introductions/SimpleArr.v
@@ -2,7 +2,7 @@ From LogRel.AutoSubst Require Import core unscoped Ast Extra.
 From LogRel Require Import Utils BasicAst Notations Context NormalForms Weakening
   GenericTyping LogicalRelation Validity.
 From LogRel.LogicalRelation Require Import Escape Reflexivity Neutral Weakening Irrelevance.
-From LogRel.Substitution Require Import Irrelevance Properties Conversion.
+From LogRel.Substitution Require Import Irrelevance Properties Conversion Reflexivity.
 From LogRel.Substitution.Introductions Require Import Universe Pi Application Lambda Var.
 
 Set Universe Polymorphism.
@@ -56,56 +56,6 @@ Section SimpleArrValidity.
     2: eapply appValid; tea.
     now bsimpl.
   Unshelve. all: tea.
-  Qed.
-
-  Lemma simple_idValid {Γ A l}
-    (VΓ : [||-v Γ])
-    {VF : [Γ ||-v<l> A | VΓ]}
-    (VΠ : [Γ ||-v<l> arr A A | VΓ]) :
-    [Γ ||-v<l> idterm A : arr A A | _ | VΠ].
-  Proof.
-    eapply irrelevanceTm'.
-    2: unshelve eapply lamValid.
-    5: unshelve eapply var0Valid.
-    - now rewrite wk1_ren_on.
-    - tea.
-  Qed.
-
-  Lemma simple_compValid {Γ A B C f g l}
-    (VΓ : [||-v Γ])
-    {VA : [Γ ||-v<l> A | VΓ]}
-    (VB : [Γ ||-v<l> B | VΓ])
-    (VC : [Γ ||-v<l> C | VΓ])
-    (VAB : [Γ ||-v<l> arr A B | VΓ])
-    (VBC : [Γ ||-v<l> arr B C | VΓ])
-    (VAC : [Γ ||-v<l> arr A C | VΓ])
-    (Vf : [Γ ||-v<l> f : arr A B | _ | VAB])
-    (Vg : [Γ ||-v<l> g : arr B C | _ | VBC]) :
-    [Γ ||-v<l> comp A g f : arr A C | _ | VAC].
-  Proof.
-    eapply irrelevanceTm'.
-    2: unshelve eapply lamValid.
-    5: unshelve eapply simple_appValid.
-    9: unshelve eapply simple_appValid.
-    13: eapply var0Valid.
-    4: eapply wk1ValidTy; exact VC.
-    4: eapply wk1ValidTy; exact VB.
-    - now rewrite wk1_ren_on.
-    - eassumption.
-    - do 2 erewrite wk1_ren_on. rewrite<- arr_ren1.
-      erewrite<- wk1_ren_on.
-      now eapply wk1ValidTy.
-    - eapply irrelevanceTm'. 2: erewrite<- wk1_ren_on;now eapply wk1ValidTm.
-      rewrite wk1_ren_on. rewrite arr_ren1.
-      do 2 rewrite wk1_ren_on. reflexivity.
-    - do 2 erewrite wk1_ren_on. rewrite<- arr_ren1.
-      erewrite<- wk1_ren_on.
-      now eapply wk1ValidTy.
-    - eapply irrelevanceTm'. 2: erewrite<- wk1_ren_on;now eapply wk1ValidTm.
-      rewrite wk1_ren_on. rewrite arr_ren1.
-      do 2 rewrite wk1_ren_on. reflexivity.
-
-      Unshelve. all: tea.
   Qed.
 
 End SimpleArrValidity.
