theories/Substitution/Reduction.v
@@ -9,14 +9,14 @@ Context `{GenericTypingProperties}.
 
 Set Printing Primitive Projection Parameters.
 
-Lemma redwfSubstValid {Γ A t u l}
+Lemma redSubstValid {Γ A t u l}
   (VΓ : [||-v Γ])
-  (red : [Γ ||-v t :⤳*: u : A | VΓ])
+  (red : [Γ ||-v t ⤳* u : A | VΓ])
   (VA : [Γ ||-v<l> A | VΓ])
   (Vu : [Γ ||-v<l> u : A | VΓ | VA]) :
   [Γ ||-v<l> t ≅ u : A | VΓ | VA].
 Proof.
-  constructor; intros. eapply redwfSubstTmEq.
+  constructor; intros. eapply redSubstLeftTmEq.
   1: now eapply validTmExt.
   now eapply validRed.
 Qed.
